guard_recursive.cpp: sketch proof

rocq-brick-libstdcpp/test/mutex/guard_recursive_cpp_proof.v
@@ -2,8 +2,69 @@ Require Import skylabs.auto.cpp.prelude.proof.
 Require Import skylabs.brick.libstdcpp.mutex.spec.
 Require Import skylabs.brick.libstdcpp.test.mutex.guard_recursive_cpp.
 
+Import linearity.
+
+Implicit Type (p : ptr) (σ : genv).
+
+Definition TT : tele := [tele (_ : Z)].
+
+#[global] Instance: Inhabited TT.
+Proof. solve_inhabited. Qed.
+
+(** Canonical "constructor" for our telescope. *)
+Polymorphic Definition mk (a : Z) : TT :=
+  {| tele_arg_head := a; tele_arg_tail := () |}.
+Succeed Definition b := recursive_mutex.Held 0 (mk 0).
+
+sl.lock
+Definition CR' `{Σ : cpp_logic, σ : genv} (a : Z) : Rep :=
+  _field "C::value" |-> intR 1$m a.
+#[only(lazy_unfold(export))] derive CR'.
+#[only(timeless)] derive CR'.
+
+(** No *)
+(* A := B *)
+(** Yes *)
+(* A := off |-> B. *)
+
+(* p
+p |->  *)
+
+sl.lock
+Definition P `{Σ : cpp_logic, σ : genv} (this : ptr) : TT -t> mpred :=
+  fun (a : Z) => this |-> CR' a.
+
+sl.lock
+Definition CR
+  `{Σ : cpp_logic, σ : genv} {HAS_THREADS : HasStdThreads Σ}
+  `{!recursive_mutex.lockedG Σ}
+  `{!HasOwn (iPropI _) recursive_mutex.cmraR}
+  (γ : recursive_mutex.rmutex_gname) (q : cQp.t) :=
+  structR "C" q **
+  _field "C::m" |-> recursive_mutex.R γ.(recursive_mutex.lock_gname) q **
+  as_Rep (fun this : ptr =>
+    recursive_mutex.inv_rmutex γ (∃ a : tele_arg TT, tele_app (P this) a)).
+
+#[only(cfractional,ascfractional,cfracvalid,type_ptr)] derive CR.
+#[only(lazy_unfold(export))] derive CR.
+
 Section with_cpp.
   Context `{Σ : cpp_logic, σ : genv} {HAS_THREADS : HasStdThreads Σ}.
+
+  Context `{!recursive_mutex.lockedG Σ}.
+  Context `{!HasOwn (iPropI _) recursive_mutex.cmraR}.
+
+  #[local] Instance: `{WeaklyObjective1 (tele_app (P p))}.
+  Proof. Admitted.
+
+  #[global] Instance P_timeless p a : Timeless (P p a).
+  Proof. rewrite P.unlock; apply _. Qed.
+
+  #[global] Instance P_timeless' p a : Timeless (tele_app (P p) a).
+  Proof. destruct a. apply _. Qed.
+
+  (* int value{0};
+  std::recursive_mutex m; *)
 
   cpp.spec "test_one_answer()" from source with (
     \post[Vint 42] emp
@@ -12,11 +73,110 @@ Section with_cpp.
     \post[Vint 42] emp
   ).
 
-  Lemma test_one_answer_ok :
-    verify?[source] "test_one_answer()".
+  Import recursive_mutex(lock_gname).
+
+  cpp.spec "C::C()" from source as C_ctor_spec with (
+    \this this
+    \persist{thr} current_thread thr
+    \post Exists γ,
+      this |-> CR γ 1$m **
+      recursive_mutex.token (lock_gname γ) 1 **
+      recursive_mutex.used_threads (lock_gname γ) {[thr]} **
+      recursive_mutex.locked (lock_gname γ) thr 0
+  ).
+
+  #[global] Instance unfold (p' : ptr) : `{AutoUnlocking.DefinedUsing (P p n) (p' |-> CR' n')} := {}.
+
+  Lemma C_ctor_ok :
+    verify[source] "C::C()".
+  Proof.
+    verify_shift; go.
+    iExists TT, (P this), (mk 0); go.
+    rewrite {1}P.unlock.
+    go.
+
+    iMod (recursive_mutex.use_thread thr (lock_gname t) ∅ with "[$]") as "?"; first set_solver.
+    iModIntro.
+    rewrite (left_id_L _ (∪)).
+    go.
+  Qed.
+
+  (* Instance: `{ShouldInlineFunction n} | 1000 := {}. *)
+  cpp.spec "C::one_answer()" from source inline.
+
+  (* cpp.spec "C::~C()" from source inline. *)
+  cpp.spec "C::~C()" from source as C_dtor_spec with (
+    \this this
+    \persist{thr} current_thread thr
+    \pre{γ} this |-> CR γ 1$m
+    \pre recursive_mutex.token (lock_gname γ) 1
+    \pre{thrs} recursive_mutex.used_threads (lock_gname γ) thrs
+    (* Currently unused, but callers are likely to have this and need to leak it. *)
+    \pre recursive_mutex.locked (lock_gname γ) thr 0
+
+    (* **
+      token (lock_gname γ) 1 **
+      used_threads (lock_gname γ) {[thr]} **
+      locked (lock_gname γ) thr 0 *)
+    \post emp).
+
+
+  Lemma C_dtor_ok :
+    (* We only get [|> recursive_mutex.dtor_spec'], and that's not enough *)
+    recursive_mutex.dtor_spec' |--
+    verify[source] "C::~C()".
   Proof.
     verify_spec; go.
-  Admitted.
+    iExists thrs; go.
+    destruct t as [? []]; rewrite P.unlock; go.
+
+    (* _now_ we just need to leak ghost state and that's okay *)
+    wname [recursive_mutex.locked] "L".
+    iApply (affine with "L").
+    apply mpred_BiAffine.
+  Qed.
+
+  cpp.spec "ghost()" from source as ghost_spec with (
+    \pre{P}
+     |={⊤}=>
+    P
+    \post P).
+
+  Lemma test_one_answer_ok :
+    verify[source] "test_one_answer()".
+  Proof.
+    verify_spec; go.
+    wname [recursive_mutex.locked (lock_gname t) thr 0] "C".
+    iAssert (recursive_mutex.acquireable (TT := TT) t thr recursive_mutex.NotHeld (P c_addr)) with "[C]" as "?". {
+      by rewrite recursive_mutex.acquireable.unlock; iFrame.
+    }
+    go.
+    rewrite P.unlock.
+    destruct args as [a []]; simpl in *.
+    go.
+
+    iExists ?[K], (mk 42).
+    go.
+    iSplitL ""; go.
+    Unset SsrIdents.
+    rename _n_ into n0.
+    Set SsrIdents.
+    (* This step breaks abstractions, but we have taken the lock yet hints don't
+    give us access to the resouce. *)
+    assert (n0 = 0 /\ n = 1)%nat as [-> ->]. {
+      rewrite-> recursive_mutex.release.unlock in *.
+      destruct n0, n; naive_solver.
+    }
+    rewrite recursive_mutex.release.unlock /=.
+    go.
+    iExists ?[K], (mk 42); go.
+    iSplitL ""; go.
+    ego with br_erefl.
+    rewrite P.unlock CR'.unlock.
+    rewrite recursive_mutex.release.unlock /=.
+    rewrite recursive_mutex.acquireable.unlock /=.
+    go.
+  Qed.
 
   Lemma test_other_answer_ok :
     verify?[source] "test_other_answer()".
